Fix more of the regression from is_trusted

SP1Chips/Lt/Constraints.lean
@@ -8,38 +8,38 @@ section constraints
 
 -- Generated Lean code for chip LtChip
 @[irreducible] def constraints (Main : Vector (Fin KB) 44) : SP1ConstraintList :=
-  let E0 : Fin KB := Main[32] + Main[32]
+  let E0 : Fin KB := Main[32] + Main[33]
   let E1 : Fin KB := Main[32] - 1
   let E2 : Fin KB := Main[32] * E1
-  let E3 : Fin KB := Main[32] - 1
-  let E4 : Fin KB := Main[32] * E3
+  let E3 : Fin KB := Main[33] - 1
+  let E4 : Fin KB := Main[33] * E3
   let E5 : Fin KB := E0 - 1
   let E6 : Fin KB := E0 * E5
-  let CS0 : SP1ConstraintList := LtOperationSigned.constraints #v[Main[15], Main[16], Main[17], Main[18]] #v[Main[25], Main[26], Main[27], Main[28]] { result := { u16_compare_operation := { bit := Main[33] }, u16_flags := #v[Main[34], Main[35], Main[36], Main[37]], not_eq_inv := Main[38], comparison_limbs := #v[Main[39], Main[40]] }, b_msb := { msb := Main[41] }, c_msb := { msb := Main[42] } } Main[32] E0
+  let CS0 : SP1ConstraintList := LtOperationSigned.constraints #v[Main[15], Main[16], Main[17], Main[18]] #v[Main[25], Main[26], Main[27], Main[28]] { result := { u16_compare_operation := { bit := Main[34] }, u16_flags := #v[Main[35], Main[36], Main[37], Main[38]], not_eq_inv := Main[39], comparison_limbs := #v[Main[40], Main[41]] }, b_msb := { msb := Main[42] }, c_msb := { msb := Main[43] } } Main[32] E0
   let E7 : Fin KB := Main[3] + 4
   let CS1 : SP1ConstraintList := CPUState.constraints { clk_high := Main[0], clk_16_24 := Main[1], clk_0_16 := Main[2], pc := #v[Main[3], Main[4], Main[5]] } #v[E7, Main[4], Main[5]] 8 E0
   let E8 : Fin KB := Main[32] * 9
-  let E9 : Fin KB := Main[32] * 10
+  let E9 : Fin KB := Main[33] * 10
   let E10 : Fin KB := E8 + E9
   let E11 : Fin KB := Main[32] * 2
-  let E12 : Fin KB := Main[32] * 3
+  let E12 : Fin KB := Main[33] * 3
   let E13 : Fin KB := E11 + E12
   let E14 : Fin KB := Main[32] * 0
-  let E15 : Fin KB := Main[32] * 0
+  let E15 : Fin KB := Main[33] * 0
   let E16 : Fin KB := E14 + E15
   let E17 : Fin KB := Main[32] * 51
-  let E18 : Fin KB := Main[32] * 51
+  let E18 : Fin KB := Main[33] * 51
   let E19 : Fin KB := E17 + E18
   let E20 : Fin KB := 32 * Main[31]
   let E21 : Fin KB := E19 - E20
   let E22 : Fin KB := Main[32] * 8
-  let E23 : Fin KB := Main[32] * 8
+  let E23 : Fin KB := Main[33] * 8
   let E24 : Fin KB := E22 + E23
   let E25 : Fin KB := 4 * Main[31]
   let E26 : Fin KB := E24 - E25
   let E27 : Fin KB := Main[1] * 65536
   let E28 : Fin KB := Main[2] + E27
-  let E29 : Fin KB := 0 + Main[33]
+  let E29 : Fin KB := 0 + Main[34]
   let CS2 : SP1ConstraintList := ALUTypeReader.constraints Main[0] E28 #v[Main[3], Main[4], Main[5]] E10 #v[E26, E21, E13, E16] #v[E29, 0, 0, 0] { op_a := Main[6], op_a_memory := { prev_value := #v[Main[7], Main[8], Main[9], Main[10]], access_timestamp := { prev_low := Main[11], diff_low_limb := Main[12] } }, op_a_0 := Main[13], op_b := Main[14], op_b_memory := { prev_value := #v[Main[15], Main[16], Main[17], Main[18]], access_timestamp := { prev_low := Main[19], diff_low_limb := Main[20] } }, op_c := #v[Main[21], Main[22], Main[23], Main[24]], op_c_memory := { prev_value := #v[Main[25], Main[26], Main[27], Main[28]], access_timestamp := { prev_low := Main[29], diff_low_limb := Main[30] } }, imm_c := Main[31] } E0
   CS0 ++ CS1 ++ CS2 ++ [
     (.assertZero E2),
