SP1Chips/Load/LoadHalf/Constraints.lean
@@ -112,16 +112,105 @@ def is_lh := Main[42] = 1
 def is_lhu := Main[43] = 1
 
 lemma allHold_constraints_iff_of_is_lh (h_is_lh : is_lh Main) :
-  List.Forall SP1Constraint.toProp (constraints Main) ↔ True := by
-  have _ := h_is_lh
-  stop
-  trivial
+  List.Forall SP1Constraint.toProp (constraints Main) ↔
+    (List.Forall SP1Constraint.toProp
+      (AddrAddOperation.constraints #v[Main[15], Main[16], Main[17], Main[18]]
+        #v[Main[21], Main[22], Main[23], Main[24]] { value := #v[Main[25], Main[26], Main[27]] } 1) ∧
+    (Main[38] = 0 ∨ Main[38] = 1) ∧
+    (Main[39] = 0 ∨ Main[39] = 1) ∧
+    (Main[28] * (Main[26] + Main[27]) = 1) ∧
+    ↑((Main[25] - 4 * Main[39] - 2 * Main[38]) * 1864368129) < 8192 ∧
+    List.Forall SP1Constraint.toProp (U16MSBOperation.constraints Main[40] { msb := Main[41] } 1) ∧
+    List.Forall SP1Constraint.toProp
+      (CPUState.constraints { clk_high := Main[0], clk_16_24 := Main[1], clk_0_16 := Main[2], pc := #v[Main[3], Main[4], Main[5]] }
+        #v[Main[3] + 4, Main[4], Main[5]] 8 1) ∧
+    List.Forall SP1Constraint.toProp
+      (ITypeReader.constraints Main[0] (Main[2] + Main[1] * 65536) #v[Main[3], Main[4], Main[5]] 30
+        #v[4, 3, 1, 0] #v[Main[40], 65535 * Main[41], 65535 * Main[41], 65535 * Main[41]]
+        { op_a := Main[6],
+          op_a_memory :=
+            { prev_value := #v[Main[7], Main[8], Main[9], Main[10]],
+              access_timestamp := { prev_low := Main[11], diff_low_limb := Main[12] } },
+          op_a_0 := Main[13], op_b := Main[14],
+          op_b_memory :=
+            { prev_value := #v[Main[15], Main[16], Main[17], Main[18]],
+              access_timestamp := { prev_low := Main[19], diff_low_limb := Main[20] } },
+          op_c_imm := #v[Main[21], Main[22], Main[23], Main[24]] } 1) ∧
+    (Main[35] = 0 ∨ Main[35] = 1) ∧
+    (Main[35] = 0 ∨ Main[0] = Main[33]) ∧
+    Main[35] * (Main[2] + Main[1] * 65536 + 1) + (1 - Main[35]) * Main[0] -
+      (Main[35] * Main[34] + (1 - Main[35]) * Main[33]) - 1 = Main[36] + Main[37] * 65536 ∧
+    ↑Main[36] < 65536 ∧
+    Main[37] < 256 ∧
+    (SP1Constraint.send
+      (AirInteraction.memory Main[33] Main[34] (Main[25] - 4 * Main[39] - 2 * Main[38])
+        Main[26] Main[27] Main[29] Main[30] Main[31] Main[32]) 1).toProp ∧
+    (SP1Constraint.receive
+      (AirInteraction.memory Main[0] (Main[2] + Main[1] * 65536 + 1)
+        (Main[25] - 4 * Main[39] - 2 * Main[38]) Main[26] Main[27] Main[29] Main[30]
+        Main[31] Main[32]) 1).toProp ∧
+    Main[43] = 0 ∧ Main[13] = 0 ∧
+    (Main[38] = 1 ∨ Main[39] = 1 ∨ Main[40] = Main[29]) ∧
+    (Main[38] = 0 ∨ Main[39] = 1 ∨ Main[40] = Main[30]) ∧
+    (Main[38] = 1 ∨ Main[39] = 0 ∨ Main[40] = Main[31]) ∧
+    (Main[38] = 0 ∨ Main[39] = 0 ∨ Main[40] = Main[32])) := by
+  have : Main[42] = 1 := h_is_lh
+  by_cases h43 : Main[43] = 0
+  · simp [constraints, AddressOperation.constraints, this, sub_eq_zero, h43]
+  · simp [constraints, AddressOperation.constraints, this, sub_eq_zero, h43]
+    intros
+    simp_all
 
 lemma allHold_constraints_iff_of_is_lhu (h_is_lhu : is_lhu Main) :
-  List.Forall SP1Constraint.toProp (constraints Main) ↔ True := by
-  have _ := h_is_lhu
-  stop
-  trivial
+  List.Forall SP1Constraint.toProp (constraints Main) ↔
+    (List.Forall SP1Constraint.toProp
+      (AddrAddOperation.constraints #v[Main[15], Main[16], Main[17], Main[18]]
+        #v[Main[21], Main[22], Main[23], Main[24]] { value := #v[Main[25], Main[26], Main[27]] } 1) ∧
+    (Main[38] = 0 ∨ Main[38] = 1) ∧
+    (Main[39] = 0 ∨ Main[39] = 1) ∧
+    (Main[28] * (Main[26] + Main[27]) = 1) ∧
+    ↑((Main[25] - 4 * Main[39] - 2 * Main[38]) * 1864368129) < 8192 ∧
+    List.Forall SP1Constraint.toProp (U16MSBOperation.constraints Main[40] { msb := Main[41] } 0) ∧
+    List.Forall SP1Constraint.toProp
+      (CPUState.constraints { clk_high := Main[0], clk_16_24 := Main[1], clk_0_16 := Main[2], pc := #v[Main[3], Main[4], Main[5]] }
+        #v[Main[3] + 4, Main[4], Main[5]] 8 1) ∧
+    List.Forall SP1Constraint.toProp
+      (ITypeReader.constraints Main[0] (Main[2] + Main[1] * 65536) #v[Main[3], Main[4], Main[5]] 33
+        #v[4, 3, 5, 0] #v[Main[40], 65535 * Main[41], 65535 * Main[41], 65535 * Main[41]]
+        { op_a := Main[6],
+          op_a_memory :=
+            { prev_value := #v[Main[7], Main[8], Main[9], Main[10]],
+              access_timestamp := { prev_low := Main[11], diff_low_limb := Main[12] } },
+          op_a_0 := Main[13], op_b := Main[14],
+          op_b_memory :=
+            { prev_value := #v[Main[15], Main[16], Main[17], Main[18]],
+              access_timestamp := { prev_low := Main[19], diff_low_limb := Main[20] } },
+          op_c_imm := #v[Main[21], Main[22], Main[23], Main[24]] } 1) ∧
+    (Main[35] = 0 ∨ Main[35] = 1) ∧
+    (Main[35] = 0 ∨ Main[0] = Main[33]) ∧
+    Main[35] * (Main[2] + Main[1] * 65536 + 1) + (1 - Main[35]) * Main[0] -
+      (Main[35] * Main[34] + (1 - Main[35]) * Main[33]) - 1 = Main[36] + Main[37] * 65536 ∧
+    ↑Main[36] < 65536 ∧
+    Main[37] < 256 ∧
+    (SP1Constraint.send
+      (AirInteraction.memory Main[33] Main[34] (Main[25] - 4 * Main[39] - 2 * Main[38])
+        Main[26] Main[27] Main[29] Main[30] Main[31] Main[32]) 1).toProp ∧
+    (SP1Constraint.receive
+      (AirInteraction.memory Main[0] (Main[2] + Main[1] * 65536 + 1)
+        (Main[25] - 4 * Main[39] - 2 * Main[38]) Main[26] Main[27] Main[29] Main[30]
+        Main[31] Main[32]) 1).toProp ∧
+    Main[42] = 0 ∧ Main[13] = 0 ∧
+    (Main[38] = 1 ∨ Main[39] = 1 ∨ Main[40] = Main[29]) ∧
+    (Main[38] = 0 ∨ Main[39] = 1 ∨ Main[40] = Main[30]) ∧
+    (Main[38] = 1 ∨ Main[39] = 0 ∨ Main[40] = Main[31]) ∧
+    (Main[38] = 0 ∨ Main[39] = 0 ∨ Main[40] = Main[32]) ∧
+    Main[41] = 0) := by
+  have : Main[43] = 1 := h_is_lhu
+  by_cases h42 : Main[42] = 0
+  · simp [constraints, AddressOperation.constraints, this, sub_eq_zero, h42]
+  · simp [constraints, AddressOperation.constraints, this, sub_eq_zero, h42]
+    intros
+    simp_all
 
 end LoadHalf
 
